README.md
@@ -1,4 +1,0 @@
-sep-logic
-=========
-
-A verification tool based on separation logic in Isabelle/HOL
